src/Sound/VCGen/Omni.dfy
@@ -1,17 +1,17 @@
 module VCGenOmni {
   import opened Defs
   import opened Context
+  import Block
   import Omni
 
-  /*method VCGen(s: Stmt, context_in: Context) returns (context: Context, VCs: seq<Expr>) 
+  method VCGen(s: Stmt, context_in: Context) returns (context: Context, VCs: seq<Expr>) 
     requires s.IsDefinedOn(|context_in.incarnation|)
     requires s.Single()
-
     ensures |context_in.incarnation| <= |context.incarnation|
     ensures (forall e <- VCs :: e.Holds()) ==> 
       forall st: State :: 
         context_in.IsSatisfiedOn(st) ==>
-        Omni.Sem(s, context_in.AdjustState(st), context.AdjustedModels)
+        Omni.SemSingle(s, context_in.AdjustState(st), context.AdjustedModels)
   {
     context := context_in;
     match s
@@ -20,7 +20,7 @@ module VCGenOmni {
       if (forall e <- VCs :: e.Holds()) {
         assert context.MkEntailment(e).Holds();
         forall st: State | context.IsSatisfiedOn(st) 
-          ensures Omni.Sem(s, context_in.AdjustState(st), context.AdjustedModels) {
+          ensures Omni.SemSingle(s, context_in.AdjustState(st), context.AdjustedModels) {
           assert context.AdjustState(st).Eval(e) by { 
             EvalConjLemma(context.ctx, st);
             context.AdjustStateSubstituteLemma(st, e);
@@ -31,7 +31,7 @@ module VCGenOmni {
       context := context_in.Add(e);
       VCs := [];
       forall st: State | context_in.IsSatisfiedOn(st) 
-        ensures Omni.Sem(s, context_in.AdjustState(st), context.AdjustedModels) {
+        ensures Omni.SemSingle(s, context_in.AdjustState(st), context.AdjustedModels) {
         if context.AdjustState(st).Eval(e) {
           context_in.SubstituteIsDefinedOnLemma(e, |st|);
           context_in.AdjustStateSubstituteLemma(st, e);
@@ -42,7 +42,7 @@ module VCGenOmni {
       vNew, context := context_in.AddEq(v, x);
       VCs := [];
       forall st: State | context_in.IsSatisfiedOn(st) 
-        ensures Omni.Sem(s, context_in.AdjustState(st), context.AdjustedModels) {
+        ensures Omni.SemSingle(s, context_in.AdjustState(st), context.AdjustedModels) {
         context_in.SubstituteIsDefinedOnLemma(x, |st|);
         var v' := st.Eval(context_in.Substitute(x));
         var st' := st + [v'];
@@ -67,79 +67,158 @@ module VCGenOmni {
           }
         }
       }
-    // case Pop => 
-    //   context := context_in.(incarnation := SeqTail(context_in.incarnation));
-    //   VCs := [];
-  }*/
+  }
 
-/*method SeqVCGen(s: seq<Stmt>, context: Context) returns (VCs: seq<Expr>) 
-  requires SeqIsDefinedOn(s, |context.incarnation|)
+  /**
+    vars n;
+      A; 
+      vars k;
+->      B; 
+        vars l;
+          C;
+        D;
+      E;
+    F
 
-  decreases SeqSize(s)
-  ensures
-    (forall e <- VCs :: e.Holds()) ==> 
-      forall st: State:: 
-        context.IsSatisfiedOn(st) ==> Omni.SeqSem(s, context.AdjustState(st), AllStates)
+
+    SeqVCGen(
+      (B; (vars l; C); D), 
+      |incr| = n + k, 
+      [(k, E); (n, F)]
+    )
+      
+   */
+
+  // function BlockWP(bcont: Block.Continuation, scont: Omni.Continuation) : iset<Omni.Continuation> 
+  //   requires |bcont| == |scont|
+  // {
+  //   iset posts: Omni.Continuation | 
+  //     && |posts| == |bcont|
+  //     && forall i: nat :: i < |bcont| ==> posts[i] 
+  // }
+
+  method SeqVCGen(s: seq<Stmt>, context: Context, bcont: Block.Continuation) returns (VCs: seq<Expr>) 
+    requires bcont.IsDefinedOn(|context.incarnation|)
+
+    requires SeqIsDefinedOn(s, bcont.AllVarsInScope())
+    requires SeqJumpsDefinedOn(s, |bcont|)
+
+    requires bcont.VarsDefined()
+    requires bcont.JumpsDefined()
+
+    decreases SeqSize(s) + bcont.Size()
+    // requires SeqIsDefinedOn(s, |context.incarnation|)
+    //requires bcont.IsDefinedOn(|context.incarnation|)
+
+    // ensures
+    //   (forall e <- VCs :: e.Holds()) ==> 
+    //     forall st: State:: 
+    //       context.IsSatisfiedOn(st) ==> 
+    //         && Omni.Sem(s, context.AdjustState(st), scont)
+    //         &&  Omni.SeqSem(s, context.AdjustState(st), AllStates)
   {
     if s == [] { 
-      VCs := []; 
-      return; 
-    }
-    var stmt, cont := s[0], s[1..];
-    assert s == [stmt] + cont;
-    SeqSizeSplitLemma(s);
-    if stmt.Single() {
-      var VCstmt, VCcont, context';
-      context', VCstmt := VCGen(stmt, context);
-      VCcont := SeqVCGen(cont, context');
-      VCs := VCstmt + VCcont;
+      if bcont == [] {
+        VCs := [];
+        return;
+      } else {
+        var varsToDelete := bcont[0].varsInScope;
+        var cont := bcont[0].cont;
+        var context' := context.Delete(varsToDelete);
+        VCs := SeqVCGen(cont, context', bcont[1..]);
+      }
     } else {
-      match stmt 
-      case Seq(ss) =>
-        SeqFunConcatLemmas(ss, cont);
-        VCs := SeqVCGen(ss + cont, context);
-        if (forall e <- VCs :: e.Holds()) {
-          forall st: State | context.IsSatisfiedOn(st) {
-            Omni.SeqLemma(ss, cont, context.AdjustState(st), AllStates);
+      var stmt, cont := s[0], s[1..];
+      assert s == [stmt] + cont;
+      SeqSizeSplitLemma(s);
+      SeqFunConcatLemmas([stmt], cont);
+      if stmt.Single() {
+        var VCstmt, VCcont, context';
+        context', VCstmt := VCGen(stmt, context) by {
+            // assume {:axiom} false;
+        }
+        VCcont := SeqVCGen(cont, context', bcont);
+        VCs := VCstmt + VCcont;
+      } else {
+        match stmt 
+        case Seq(ss) =>
+          VCs := SeqVCGen(ss + cont, context, bcont) by {
+            // decreases
+            SeqFunConcatLemmas(ss, cont);
           }
-        }
-      case Choice(ss0, ss1) =>
-        var VCs0 := SeqVCGen([ss0] + cont, context);
-        var VCs1 := SeqVCGen([ss1] + cont, context);
-        VCs := VCs0 + VCs1;
-      case VarDecl(v, s) =>
-        var vNew, context' := context.AddVar();
-        VCs := SeqVCGen([s] + WithPop(cont), context') by {
-          SeqFunConcatLemmas([Pop], cont);
-        }
-        if (forall e <- VCs :: e.Holds()) {
-          forall st: State | context.IsSatisfiedOn(st)
-            ensures Omni.SeqSem([VarDecl(v, s)] + cont, context.AdjustState(st), AllStates) {
-            Omni.SemNest(VarDecl(v, s), cont, context.AdjustState(st), AllStates) by {
-              forall b: Value ensures Omni.Sem(s, context.AdjustState(st).Update(b), 
-                UpdateSet(Omni.SeqWP(cont, AllStates)))
-              { 
-                assert context.AdjustState(st).Update(b) == context'.AdjustState(st + [b]);
-                assert context'.IsSatisfiedOn(st + [b]) by {
-                  forall e <- context'.ctx 
-                    ensures (st + [b]).Eval(e) {
-                      e.EvalDepthLemma(st, st + [b]);
-                  }
-                }
-                Omni.SemCons(s, context.AdjustState(st).Update(b), 
-                  Omni.SeqWP(WithPop(cont), AllStates), 
-                  UpdateSet(Omni.SeqWP(cont, AllStates))) by 
-                {
-                  forall st | Omni.SeqSem(WithPop(cont), st, AllStates) 
-                    ensures Omni.SeqSem(cont, Tail(st), AllStates) {
-                    Omni.SeqFrameLemmaAll(cont, v, st);
-                  }
-                }
-              }
-            }
+        case Choice(ss0, ss1) =>
+          var VCs0 := SeqVCGen([ss0] + cont, context, bcont);
+          var VCs1 := SeqVCGen([ss1] + cont, context, bcont);
+          VCs := VCs0 + VCs1;
+        case NewScope(n, body) =>
+          var context' := context.AddVars(n);
+          VCs := SeqVCGen([body], context', bcont.Update(cont, n)) by {
+            // decreases
+            bcont.UpdateSize(cont, n);
+            assert SeqSize([body]) == body.Size();
           }
-        }
-      case WithPop(ss) => assume {:axiom} false;
+        case Escape(l) =>
+          var varsToDelete := bcont.VarsInScope(l);
+          var context' := context.Delete(varsToDelete) by {
+            bcont.VarsInScopeLeqAll(l);
+          }
+          VCs := SeqVCGen([], context', bcont[l..]) by {
+            // decreases
+            bcont.SizePrefix(l);
+            // IsDefinedOn
+            bcont.VarsInScopeLeqAll(l);
+            // JumpsDefined
+            bcont.DefinedPrefix(l);
+          }
+      }
     }
-  }*/
+  }
 }
+
+      
+      // match stmt 
+      // case Seq(ss) =>
+      //   SeqFunConcatLemmas(ss, cont);
+      //   VCs := SeqVCGen(ss + cont, context);
+      //   if (forall e <- VCs :: e.Holds()) {
+      //     forall st: State | context.IsSatisfiedOn(st) {
+      //       Omni.SeqLemma(ss, cont, context.AdjustState(st), AllStates);
+      //     }
+      //   }
+      // case Choice(ss0, ss1) =>
+      //   var VCs0 := SeqVCGen([ss0] + cont, context);
+      //   var VCs1 := SeqVCGen([ss1] + cont, context);
+      //   VCs := VCs0 + VCs1;
+      // case VarDecl(v, s) =>
+      //   var vNew, context' := context.AddVar();
+      //   VCs := SeqVCGen([s] + [WithPop(cont)], context') by {
+      //     SeqFunConcatLemmas([s], [WithPop(cont)]);
+      //   }
+      //   if (forall e <- VCs :: e.Holds()) {
+      //     forall st: State | context.IsSatisfiedOn(st)
+      //       ensures Omni.SeqSem([VarDecl(v, s)] + cont, context.AdjustState(st), AllStates) {
+      //       Omni.SemNest(VarDecl(v, s), cont, context.AdjustState(st), AllStates) by {
+      //         forall b: Value ensures Omni.Sem(s, context.AdjustState(st).Update(b), 
+      //           UpdateSet(Omni.SeqWP(cont, AllStates)))
+      //         { 
+      //           assert context.AdjustState(st).Update(b) == context'.AdjustState(st + [b]);
+      //           assert context'.IsSatisfiedOn(st + [b]) by {
+      //             forall e <- context'.ctx 
+      //               ensures (st + [b]).Eval(e) {
+      //                 e.EvalDepthLemma(st, st + [b]);
+      //             }
+      //           }
+      //           Omni.SemCons(s, context.AdjustState(st).Update(b), 
+      //             Omni.SeqWP([WithPop(cont)], AllStates), 
+      //             UpdateSet(Omni.SeqWP(cont, AllStates))) by 
+      //           {
+      //             forall st | Omni.SeqSem([WithPop(cont)], st, AllStates) 
+      //               ensures Omni.SeqSem(cont, Tail(st), AllStates) {
+      //               Omni.SeqFrameLemmaAll(cont, v, st);
+      //             }
+      //           }
+      //         }
+      //       }
+      //     }
+      //   }
+ 
